bruh is this even right lol

proof.v
@@ -11,7 +11,7 @@ Set Implicit Arguments.
 Inductive OpType : Set :=
   | Plus.
 
-Definition Id : nat.
+Definition Id := nat.
 (* var, time -> val *)
 Definition env := string -> nat -> nat.
 Definition time := nat.
@@ -19,17 +19,17 @@ Definition time := nat.
 Inductive node : Set :=
   | BV (b : nat)
   | Var (s : string)
-  | Op (o : OpType) (e1 : nat) (e2 : nat)
+  | Op (o : OpType) (e1 : Id) (e2 : Id)
   | Reg (regid : nat) (init : nat).
   
 Definition prog := list (node).
 
 (* Ltac --> interpreter, starter code for some homework thing in 505 *)
 (* index is a function that takes an id and a program, and returns the node at p[i] *)
-Fixpoint index (i : nat) (p : prog) : node :=
+Fixpoint index (i : nat) (p : prog) : option node :=
   match (i, p) with
-    | (_, []) => (Var "error")
-    | (0, (n :: _)) => n
+    | (_, []) => None
+    | (0, (n :: _)) => (Some n)
     | (S n, p) => index n (tl p)
   end.
 
@@ -37,17 +37,27 @@ Fixpoint index (i : nat) (p : prog) : node :=
 
 (* step : prog -> env -> id -> time -> bv -> Prop *)
 Inductive step : prog -> env -> nat -> time -> nat -> Prop :=
-| step_bv : forall p env id t b,
-    step p env id t b
+| step_bv :
+  forall p env id t b,
+    index id p = Some (BV b) ->
+      step p env id t b
 | step_var : forall p env id t x,
-    step p env id t (env x t)
+    index id p = Some (Var x) ->
+      step p env id t (env x t)
 | step_op : forall p env id t e1 e2 v1 v2,  
+    index id p = Some (Op Plus e1 e2) ->
     step p env e1 t v1 ->
     step p env e2 t v2 ->
     step p env id t (v1 + v2) 
-| step_reg : forall p env id t n init, 
-    step p env n t init ->
-    (t = 0 -> step p env id t init \/ t > 0 -> step p env id (t - 1) 0).
+| step_reg_init : forall p env id t n init, 
+    t = 0 ->
+    index id p = Some (Reg n init) ->
+    step p env id t init
+| step_reg : forall p env id t n init b, 
+    index id p = Some (Reg n init) ->
+    t > 0 ->
+    step p env n t b ->
+    step p env id t b.
 
 Lemma check_simple_comb_output :
   let prog := [(Op Plus 1 2) ; (BV 1) ; (BV 2)] in
@@ -57,12 +67,43 @@ Lemma check_simple_comb_output :
     step prog env id_num t 3.
 Proof.
   intros.
-  unfold prog.
+  unfold prog0.
   unfold env.
   unfold id_num.
   apply step_op with (e1 := 1) (e2 := 2) (v1 := 1) (v2 := 2).
   - constructor.
-  - apply step_bv.
-  Qed.
+  - apply step_bv. unfold index. simpl. reflexivity.
+  - apply step_bv. unfold index. simpl. reflexivity.
+Qed.
 
+Lemma simple_equiv_check :
+  let prog1 := [(Reg 1 0) ; (Op Plus 2 3) ; (BV 1) ; (BV 2)] in
+  let prog2 := [(Op Plus 1 2) ; (Reg 3 0) ; (Reg 4 0) ; (BV 1) ; (BV 2)] in
+  let id_num := 0 in
+  forall env t,
+    t > 1 ->
+    exists b, step prog1 env id_num t b /\ step prog2 env id_num t b.
+Proof.
+  intros. 
+  eexists ?[b].
+  unfold id_num.
+  econstructor.
+  - apply step_reg with (n := 1) (init := 0) (b := 3).
+    + simpl. reflexivity.
+    + lia.
+    + unfold prog1. apply step_op with (p := prog1) (env := env0) (t := t) (id := 1) (e1 := 2) (e2 := 3) (v1 := 1) (v2 := 2).
+     * simpl. reflexivity.
+     * econstructor. simpl. reflexivity.
+     * econstructor. simpl. reflexivity.
+  - apply step_op with (p := prog2) (env := env0) (t := t) (id := 0) (e1 := 1) (e2 := 2) (v1 := 1) (v2 := 2).
+    + simpl. reflexivity.
+    + apply step_reg with (p := prog2) (env := env0) (t := t) (n := 3) (init := 0) (b := 1).
+      * simpl. reflexivity.
+      * lia.
+      * econstructor. simpl. reflexivity.
+    + apply step_reg with (p := prog2) (env := env0) (t := t) (n := 4) (init := 0) (b := 2).
+      * simpl. reflexivity.
+      * lia.
+      * econstructor. simpl. reflexivity.
+  Qed.
 
